{
 "cells": [
  {
   "cell_type": "markdown",
   "id": "c2506cb0",
   "metadata": {},
   "source": [
    "# $SU(3)$ one-body reduced matrix elements acting on different shells"
   ]
  },
  {
   "cell_type": "markdown",
   "id": "c48e2846",
   "metadata": {},
   "source": [
    "\n",
    "# 1. Downwards transition $\\eta>\\eta'$\n",
    "<ul>\n",
    "<li>Uncoupling of the complete matrix element and application of Wigner-Eckart theorem. Notice that the Wigner-Eckart theorem convention is not to put any $1/\\sqrt{2L+1}$ coefficients. \n",
    "\n",
    "$$\\Big\\langle[f'_-]\\otimes[f'_+],(\\lambda'_-\\mu'_-)\\otimes(\\lambda'_+\\mu'_+),\\rho'(\\lambda'\\mu'),K',L',M_{L'},S',M_{S'}\\Big|\\\\\\times\\big\\{a^{\\dagger}_{(\\eta'0)\\frac{1}{2}}\\tilde{a}_{(0\\eta)\\frac{1}{2}}\\big\\}^{\\rho_0=1,(\\lambda_0\\mu_0)K_0L_0S_0}_{\\hspace{17mm}M_{L_0}M_{S_0}}\n",
    "\\\\\\times\\Big|[f_-]\\otimes[f_+],(\\lambda_-\\mu_-)\\otimes(\\lambda_+\\mu_+),\\rho(\\lambda\\mu),K,L,M_{L},S,M_{S}\\Big\\rangle \n",
    "\\\\\\\\= \\sum_{\\substack{K'_{-}, L'_{-},M_{L'_{-}},K'_{+}, L'_{+},M_{L'_{+}},S'_-,M_{S'_{-}},S'_+,M_{S'_{+}} \\\\ l',m_{l'},m_{s'},l,m_l,m_s \\\\ K_{-}, L_{-},M_{L_{-}},K_{+}, L_{+},M_{L_{+}},S_-,M_{S_{-}},S_+,M_{S_{+}}}} \n",
    "\\\\\\langle(\\lambda'_-\\mu'_-),K'_-,L'_-; (\\lambda'_+\\mu'_+),K'_+,L'_+||(\\lambda'\\mu'),K',L'\\rangle_{\\rho'}\n",
    "\\langle L'_-,M_{L'_-},L'_+,M_{L'_+}|L',M_{L'}\\rangle  \\langle S'_-,M_{S'_-},S'_+,M_{S'_+}|S',M_{S'}\\rangle\n",
    "\\\\\\times\\langle(\\eta',0),0,l'; (0,\\eta),0,l||(\\lambda_o\\mu_o),K_o,L_o\\rangle_{\\rho_o=1}\n",
    "\\langle l',m_{l'},l,m_{l}|L_o,M_{L_o}\\rangle  \\langle \\frac{1}{2},m_{s'},\\frac{1}{2},m_{s}|S_o,M_{S_o}\\rangle\n",
    "\\\\\\times\\langle(\\lambda_-\\mu_-),K_-,L_-; (\\lambda_+\\mu_+),K_+,L_+||(\\lambda\\mu),K,L\\rangle_{\\rho}\n",
    "\\langle L_-,M_{L_-},L_+,M_{L_+}|L,M_{L}\\rangle  \\langle S_-,M_{S_-},S_+,M_{S_+}|S,M_{S}\\rangle\n",
    "\\\\\\times\\Big\\langle[f'_-],(\\lambda'_-\\mu'_-),K'_-,L'_-,M_{L'_-},S'_-,M_{S'_-}\\Big|a^{\\dagger}_{(\\eta'0),0,l',m_{l'}\\frac{1}{2},m_{s'}}\\Big| [f_-],(\\lambda_-\\mu_-),K_-,L_-,M_{L_-},S_-,M_{S_-}\\Big\\rangle\n",
    "\\\\\\times\\Big\\langle [f'_+],(\\lambda'_+\\mu'_+),K'_+,L'_+,M_{L'_+},S'_+,M_{S'_+} \\Big|\\tilde{a}_{(0\\eta),0,l,m_{l}\\frac{1}{2},m_{s}}\\Big|[f_+],(\\lambda_+\\mu_+),K_+,L_+,M_{L_+},S_+,M_{S_+}\\Big\\rangle\n",
    "\\\\\\\\= \\sum_{\\substack{K'_{-}, L'_{-},M_{L'_{-}},K'_{+}, L'_{+},M_{L'_{+}},S'_-,M_{S'_{-}},S'_+,M_{S'_{+}} \\\\ l',m_{l'},m_{s'},l,m_l,m_s \\\\ K_{-}, L_{-},M_{L_{-}},K_{+}, L_{+},M_{L_{+}},S_-,M_{S_{-}},S_+,M_{S_{+}}}} \n",
    "\\\\\\langle(\\lambda'_-\\mu'_-),K'_-,L'_-; (\\lambda'_+\\mu'_+),K'_+,L'_+||(\\lambda'\\mu'),K',L'\\rangle_{\\rho'}\n",
    "\\langle L'_-,M_{L'_-},L'_+,M_{L'_+}|L',M_{L'}\\rangle  \\langle S'_-,M_{S'_-},S'_+,M_{S'_+}|S',M_{S'}\\rangle\n",
    "\\\\\\times\\langle(\\eta',0),0,l'; (0,\\eta),0,l||(\\lambda_o\\mu_o),K_o,L_o\\rangle_{\\rho_o=1}\n",
    "\\langle l',m_{l'},l,m_{l}|L_o,M_{L_o}\\rangle  \\langle \\frac{1}{2},m_{s'},\\frac{1}{2},m_{s}|S_o,M_{S_o}\\rangle\n",
    "\\\\\\times\\langle(\\lambda_-\\mu_-),K_-,L_-; (\\lambda_+\\mu_+),K_+,L_+||(\\lambda\\mu),K,L\\rangle_{\\rho}\n",
    "\\langle L_-,M_{L_-},L_+,M_{L_+}|L,M_{L}\\rangle  \\langle S_-,M_{S_-},S_+,M_{S_+}|S,M_{S}\\rangle\n",
    "\\\\\\times\\langle(\\lambda_-\\mu_-),K_-,L_-; (\\eta'0),0, l'||(\\lambda'_-\\mu'_-),K'_-,L'_-\\rangle_{\\rho=1}\\langle L_-,M_{L_-},l',m_{l'}|L'_-,M_{L'_-}\\rangle\\langle S_-,M_{S_-},\\frac{1}{2},m_{s'}|S'_-,M_{S'_-}\\rangle\n",
    "\\\\\\times\\Big\\langle[f'_-],(\\lambda'_-\\mu'_-),S'_-\\Big|\\Big|\\Big|a^{\\dagger}_{(\\eta'0)\\frac{1}{2}}\\Big|\\Big|\\Big| [f_-],(\\lambda_-\\mu_-)S_-\\Big\\rangle_{\\rho=1}\n",
    "\\\\\\times\\langle(\\lambda_+\\mu_+),K_+,L_+; (0\\eta),0, l||(\\lambda'_+\\mu'_+),K'_+,L'_+\\rangle_{\\rho=1}\\langle L_+,M_{L_+},l,m_{l}|L'_+,M_{L'_+}\\rangle\\langle S_+,M_{S_+},\\frac{1}{2},m_{s}|S'_+,M_{S'_+}\\rangle\n",
    "\\\\\\times\\Big\\langle [f'_+],(\\lambda'_+\\mu'_+),S'_+\\Big|\\Big|\\Big|\\tilde{a}_{(0\\eta),\\frac{1}{2}}\\Big|\\Big|\\Big|[f_+],(\\lambda_+\\mu_+),S_+\\Big\\rangle_{\\rho=1}\\\\\n",
    "$$\n",
    "    \n",
    "   \n",
    " "
   ]
  },
  {
   "cell_type": "markdown",
   "id": "7dbe60f2",
   "metadata": {},
   "source": [
    "\n",
    "<li>Apply Wigner-Eckart theorem on the left hand side \n",
    "    \n",
    "$$ \n",
    "\\Big\\langle[f'_-]\\otimes[f'_+],(\\lambda'_-\\mu'_-)\\otimes(\\lambda'_+\\mu'_+),\\rho'(\\lambda'\\mu'),K',L',M_{L'},S',M_{S'}\\Big|\\\\\\times\\big\\{a^{\\dagger}_{(\\eta'0)\\frac{1}{2}}\\tilde{a}_{(0\\eta)\\frac{1}{2}}\\big\\}^{\\rho_0=1,(\\lambda_0\\mu_0)K_0L_0S_0}_{\\hspace{17mm}M_{L_0}M_{S_0}}\n",
    "\\\\\\times\\Big|[f_-]\\otimes[f_+],(\\lambda_-\\mu_-)\\otimes(\\lambda_+\\mu_+),\\rho(\\lambda\\mu),K,L,M_{L},S,M_{S}\\Big\\rangle\n",
    "\\\\= \\sum_{\\bar{\\rho}} \\langle(\\lambda\\mu),K,L;(\\lambda_o\\mu_o)K_oL_o ||(\\lambda'\\mu'),K',L'\\rangle_{\\bar{\\rho}}\n",
    "\\langle LM_{L}L_oM_{L_o}|L'M_{L'}\\rangle\n",
    "\\langle SM_{S}S_oM_{S_o}|S'M_{S'}\\rangle\n",
    "\\\\\\times\\Big\\langle[f'_-]\\otimes[f'_+],(\\lambda'_-\\mu'_-)\\otimes(\\lambda'_+\\mu'_+),\\rho'(\\lambda'\\mu'),S'\\Big|\\Big|\\Big| \\big\\{a^{\\dagger}_{(\\eta'0)\\frac{1}{2}}\\tilde{a}_{(0\\eta)\\frac{1}{2}}\\big\\}^{\\rho_0=1,(\\lambda_0\\mu_0)S_0}\\Big|\\Big|\\Big|[f_-]\\otimes[f_+],(\\lambda_-\\mu_-)\\otimes(\\lambda_+\\mu_+),\\rho(\\lambda\\mu),S\\Big\\rangle_{\\bar{\\rho}}\\\\\\\\\\\\\n",
    "$$\n",
    "    \n"
   ]
  },
  {
   "cell_type": "markdown",
   "id": "5f28e14c",
   "metadata": {},
   "source": [
    "\n",
    "<li>Multiply by $\\sum_{K,L,K_o,L_o} \\langle(\\lambda\\mu),K,L;(\\lambda_o\\mu_o)K_oL_o ||(\\lambda'\\mu'),K',L'\\rangle_{\\bar{\\rho}}$ and apply $SU(3)$ orthogonality relations in the left hand side. Multiply by $\\sum_{M_L,M_{L_o}}\\langle LM_{L}L_oM_{L_o}|L'M_{L'}\\rangle$ and $\\sum_{M_S,M_{S_o}}\\langle SM_{S}S_oM_{S_o}|S'M_{S'}\\rangle$. Apply orthogonality and group the $SU(3)$, $SO(3)$ and $SU(2)$ coefficients.\n",
    "    \n",
    "$$  \n",
    "\\Big\\langle[f'_-]\\otimes[f'_+],(\\lambda'_-\\mu'_-)\\otimes(\\lambda'_+\\mu'_+),\\rho'(\\lambda'\\mu'),S'\\Big|\\Big|\\Big| \\big\\{a^{\\dagger}_{(\\eta'0)\\frac{1}{2}}\\tilde{a}_{(0\\eta)\\frac{1}{2}}\\big\\}^{\\rho_0=1,(\\lambda_0\\mu_0)S_0}\\Big|\\Big|\\Big|[f_-]\\otimes[f_+],(\\lambda_-\\mu_-)\\otimes(\\lambda_+\\mu_+),\\rho(\\lambda\\mu),S\\Big\\rangle_{\\bar{\\rho}}\n",
    "\\\\= \\sum_{\\substack{K'_{-}, L'_{-},M_{L'_{-}},K'_{+}, L'_{+},M_{L'_{+}},S'_-,M_{S'_{-}},S'_+,M_{S'_{+}} \\\\ l',m_{l'},m_{s'},l,m_l,m_s \\\\ K_{-}, L_{-},M_{L_{-}},K_{+}, L_{+},M_{L_{+}},S_-,M_{S_{-}},S_+,M_{S_{+}} \\\\ K,L,K_o,L_o,M_L,M_{L_o},M_S,M_{S_o} }} \n",
    "\\\\\\langle(\\lambda'_-\\mu'_-),K'_-,L'_-; (\\lambda'_+\\mu'_+),K'_+,L'_+||(\\lambda'\\mu'),K',L'\\rangle_{\\rho'}\n",
    "\\langle L'_-,M_{L'_-},L'_+,M_{L'_+}|L',M_{L'}\\rangle  \\langle S'_-,M_{S'_-},S'_+,M_{S'_+}|S',M_{S'}\\rangle\n",
    "\\\\\\times\\langle(\\eta',0),0,l'; (0,\\eta),0,l||(\\lambda_o\\mu_o),K_o,L_o\\rangle_{\\rho_o=1}\n",
    "\\langle l',m_{l'},l,m_{l}|L_o,M_{L_o}\\rangle  \\langle \\frac{1}{2},m_{s'},\\frac{1}{2},m_{s}|S_o,M_{S_o}\\rangle\n",
    "\\\\\\times\\langle(\\lambda_-\\mu_-),K_-,L_-; (\\lambda_+\\mu_+),K_+,L_+||(\\lambda\\mu),K,L\\rangle_{\\rho}\n",
    "\\langle L_-,M_{L_-},L_+,M_{L_+}|L,M_{L}\\rangle  \\langle S_-,M_{S_-},S_+,M_{S_+}|S,M_{S}\\rangle\n",
    "\\\\\\times\\langle(\\lambda_-\\mu_-),K_-,L_-; (\\eta'0),0, l'||(\\lambda'_-\\mu'_-),K'_-,L'_-\\rangle_{\\rho=1}\\langle L_-,M_{L_-},l',m_{l'}|L'_-,M_{L'_-}\\rangle\\langle S_-,M_{S_-},\\frac{1}{2},m_{s'}|S'_-,M_{S'_-}\\rangle\n",
    "\\\\\\times\\Big\\langle[f'_-],(\\lambda'_-\\mu'_-),S'_-\\Big|\\Big|\\Big|a^{\\dagger}_{(\\eta'0)\\frac{1}{2}}\\Big|\\Big|\\Big| [f_-],(\\lambda_-\\mu_-)S_-\\Big\\rangle_{\\rho=1}\n",
    "\\\\\\times\\langle(\\lambda_+\\mu_+),K_+,L_+; (0\\eta),0, l||(\\lambda'_+\\mu'_+),K'_+,L'_+\\rangle_{\\rho=1}\\langle L_+,M_{L_+},l,m_{l}|L'_+,M_{L'_+}\\rangle\\langle S_+,M_{S_+},\\frac{1}{2},m_{s}|S'_+,M_{S'_+}\\rangle\n",
    "\\\\\\times\\Big\\langle [f'_+],(\\lambda'_+\\mu'_+),S'_+\\Big|\\Big|\\Big|\\tilde{a}_{(0\\eta),\\frac{1}{2}}\\Big|\\Big|\\Big|[f_+],(\\lambda_+\\mu_+),S_+\\Big\\rangle_{\\rho=1}\\\\\n",
    "\\times \\langle(\\lambda\\mu),K,L;(\\lambda_o\\mu_o)K_oL_o ||(\\lambda'\\mu'),K',L'\\rangle_{\\bar{\\rho}}\\langle LM_{L}L_oM_{L_o}|L'M_{L'}\\rangle \\langle SM_{S}S_oM_{S_o}|S'M_{S'}\\rangle\n",
    "\\\\\\\\\\\\\\\\=\n",
    "\\sum_{\\substack{K'_{-}, L'_{-},K'_{+}, L'_{+} \\\\ l',l \\\\ K_{-}, L_{-},,K_{+}, L_{+}\\\\ K,L,K_o,L_o}} \n",
    "\\\\\\times\\langle(\\lambda'_-\\mu'_-),K'_-,L'_-; (\\lambda'_+\\mu'_+),K'_+,L'_+||(\\lambda'\\mu'),K',L'\\rangle_{\\rho'}\n",
    "\\\\\\times\\langle(\\eta',0),0,l'; (0,\\eta),0,l||(\\lambda_o\\mu_o),K_o,L_o\\rangle_{\\rho_o=1}\n",
    "\\\\\\times\\langle(\\lambda_-\\mu_-),K_-,L_-; (\\lambda_+\\mu_+),K_+,L_+||(\\lambda\\mu),K,L\\rangle_{\\rho}\n",
    "\\\\\\times\\langle(\\lambda_-\\mu_-),K_-,L_-; (\\eta'0),0, l'||(\\lambda'_-\\mu'_-),K'_-,L'_-\\rangle_{\\rho=1}\n",
    "\\\\\\times\\langle(\\lambda_+\\mu_+),K_+,L_+; (0\\eta),0, l||(\\lambda'_+\\mu'_+),K'_+,L'_+\\rangle_{\\rho=1}\n",
    "\\\\\\times\\langle(\\lambda\\mu),K,L;(\\lambda_o\\mu_o)K_oL_o ||(\\lambda'\\mu'),K',L'\\rangle_{\\bar{\\rho}}\n",
    "\\\\\\\\\\sum_{\\substack{M_{L'_{-}},M_{L'_{+}} \\\\ m_{l'},m_l, M_{L_{-}},M_{L_{+}}, M_L,M_{L_o} }} \n",
    "\\\\\\times\\langle L'_-,M_{L'_-},L'_+,M_{L'_+}|L',M_{L'}\\rangle\n",
    "\\\\\\times\\langle l',m_{l'},l,m_{l}|L_o,M_{L_o}\\rangle\n",
    "\\\\\\times\\langle L_-,M_{L_-},L_+,M_{L_+}|L,M_{L}\\rangle  \n",
    "\\\\\\times\\langle L_-,M_{L_-},l',m_{l'}|L'_-,M_{L'_-}\\rangle\n",
    "\\\\\\times\\langle L_+,M_{L_+},l,m_{l}|L'_+,M_{L'_+}\\rangle\n",
    "\\\\\\times\\langle LM_{L}L_oM_{L_o}|L'M_{L'}\\rangle\n",
    "\\\\\\\\\\sum_{\\substack{S'_-,M_{S'_{-}},S'_+,M_{S'_{+}} \\\\ m_{s'},m_s, S_-,M_{S_{-}},S_+,M_{S_{+}},M_S,M_{S_o} }} \n",
    "\\\\\\times\\langle S'_-,M_{S'_-},S'_+,M_{S'_+}|S',M_{S'}\\rangle\n",
    "\\\\\\times\\langle \\frac{1}{2},m_{s'},\\frac{1}{2},m_{s}|S_o,M_{S_o}\\rangle\n",
    "\\\\\\times\\langle S_-,M_{S_-},S_+,M_{S_+}|S,M_{S}\\rangle\n",
    "\\\\\\times\\langle S_-,M_{S_-},\\frac{1}{2},m_{s'}|S'_-,M_{S'_-}\\rangle\n",
    "\\\\\\times\\langle S_+,M_{S_+},\\frac{1}{2},m_{s}|S'_+,M_{S'_+}\\rangle\n",
    "\\\\\\times\\langle SM_{S}S_oM_{S_o}|S'M_{S'}\\rangle\n",
    "\\\\\\\\\\times \\Big\\langle[f'_-],(\\lambda'_-\\mu'_-),S'_-\\Big|\\Big|\\Big|a^{\\dagger}_{(\\eta'0)\\frac{1}{2}}\\Big|\\Big|\\Big| [f_-],(\\lambda_-\\mu_-)S_-\\Big\\rangle_{\\rho=1}\\Big\\langle [f'_+],(\\lambda'_+\\mu'_+),S'_+\\Big|\\Big|\\Big|\\tilde{a}_{(0\\eta),\\frac{1}{2}}\\Big|\\Big|\\Big|[f_+],(\\lambda_+\\mu_+),S_+\\Big\\rangle_{\\rho=1}\n",
    "$$    \n",
    "    \n",
    "\n",
    "  "
   ]
  },
  {
   "cell_type": "markdown",
   "id": "a15b6272",
   "metadata": {},
   "source": [
    "\n",
    "<li> The grouped summations are the unitary 9-j symbols. No sum over $ S'_-,S'_+, S_-,S_+$ will appear since these labels are fixed by the irreps $[f'_-],[f'_+],[f_-],[f_+]$ respectively\n",
    "    \n",
    "$$  \n",
    "\\boxed{\n",
    "\\Big\\langle[f'_-]\\otimes[f'_+],(\\lambda'_-\\mu'_-)\\otimes(\\lambda'_+\\mu'_+),\\rho'(\\lambda'\\mu'),S'\\Big|\\Big|\\Big| \\big\\{a^{\\dagger}_{(\\eta'0)\\frac{1}{2}}\\tilde{a}_{(0\\eta)\\frac{1}{2}}\\big\\}^{\\rho_0=1,(\\lambda_0\\mu_0)S_0}\\Big|\\Big|\\Big|[f_-]\\otimes[f_+],(\\lambda_-\\mu_-)\\otimes(\\lambda_+\\mu_+),\\rho(\\lambda\\mu),S\\Big\\rangle_{\\bar{\\rho}}\n",
    "\\\\= \\begin{Bmatrix}\n",
    "  (\\lambda_-,\\mu_-) & (\\eta',0) & (\\lambda'_-,\\mu'_-) & \\rho=1\\\\\n",
    "  (\\lambda_+,\\mu_+) & (0,\\eta) & (\\lambda'_+,\\mu'_+) & \\rho=1\\\\\n",
    "  (\\lambda,\\mu) & (\\lambda_o,\\mu_o) & (\\lambda',\\mu') & \\bar{\\rho}\\\\\n",
    "  \\rho & \\rho=1 & \\rho'&\n",
    " \\end{Bmatrix}\n",
    "\\chi\\begin{Bmatrix}\n",
    "  S_- & \\frac{1}{2} & S'_- \\\\\n",
    "  S_+ & \\frac{1}{2} & S'_+ \\\\\n",
    "  S & S_o & S' \\\\\n",
    " \\end{Bmatrix}\n",
    "\\\\\\\\ \\times\\Big\\langle[f'_-],(\\lambda'_-\\mu'_-),S'_-\\Big|\\Big|\\Big|a^{\\dagger}_{(\\eta'0)\\frac{1}{2}}\\Big|\\Big|\\Big| [f_-],(\\lambda_-\\mu_-)S_-\\Big\\rangle_{\\rho=1}\\Big\\langle [f'_+],(\\lambda'_+\\mu'_+),S'_+\\Big|\\Big|\\Big|\\tilde{a}_{(0\\eta),\\frac{1}{2}}\\Big|\\Big|\\Big|[f_+],(\\lambda_+\\mu_+),S_+\\Big\\rangle_{\\rho=1}\n",
    "}\n",
    "$$    \n",
    "    \n",
    "This is an extension of equation 6 in J. Millener, Su(3) in shell-model calculations (1991) including spin labels."
   ]
  },
  {
   "cell_type": "markdown",
   "id": "6cba1dbc",
   "metadata": {},
   "source": [
    "<li> Using the relation\n",
    "    \n",
    "$$\n",
    "\\Big\\langle[f''](\\lambda''\\mu''),S''\\Big|\\Big|\\Big|\\tilde{a}_{(0\\eta)\\frac{1}{2}}\\Big|\\Big|\\Big|[f](\\lambda\\mu),S\\Big\\rangle_{\\rho=1}\n",
    "= (-1)^{\\eta+\\frac{1}{2}+S-S''+\\lambda''-\\lambda+\\mu''-\\mu}\\sqrt{\\frac{\\text{dim}(\\lambda\\mu)}{\\text{dim}(\\lambda''\\mu'')}}\\sqrt{\\frac{2S+1}{2S''+1}}\\Big\\langle[f](\\lambda\\mu),S\\Big|\\Big|\\Big|a^{\\dagger}_{(\\eta0)\\frac{1}{2}}\\Big|\\Big|\\Big|[f''](\\lambda''\\mu''),S''\\Big\\rangle_{\\rho=1}\n",
    "$$\n",
    "\n"
   ]
  },
  {
   "cell_type": "markdown",
   "id": "619aca4b",
   "metadata": {},
   "source": [
    "abvoe which results in \n",
    "    \n",
    "$$  \n",
    "\\boxed{\n",
    "\\Big\\langle[f'_-]\\otimes[f'_+],(\\lambda'_-\\mu'_-)\\otimes(\\lambda'_+\\mu'_+),\\rho'(\\lambda'\\mu'),S'\\Big|\\Big|\\Big| \\big\\{a^{\\dagger}_{(\\eta'0)\\frac{1}{2}}\\tilde{a}_{(0\\eta)\\frac{1}{2}}\\big\\}^{\\rho_0=1,(\\lambda_0\\mu_0)S_0}\\Big|\\Big|\\Big|[f_-]\\otimes[f_+],(\\lambda_-\\mu_-)\\otimes(\\lambda_+\\mu_+),\\rho(\\lambda\\mu),S\\Big\\rangle_{\\bar{\\rho}}\n",
    "\\\\= \\begin{Bmatrix}\n",
    "  (\\lambda_-,\\mu_-) & (\\eta',0) & (\\lambda'_-,\\mu'_-) & \\rho=1\\\\\n",
    "  (\\lambda_+,\\mu_+) & (0,\\eta) & (\\lambda'_+,\\mu'_+) & \\rho=1\\\\\n",
    "  (\\lambda,\\mu) & (\\lambda_o,\\mu_o) & (\\lambda',\\mu') & \\bar{\\rho}\\\\\n",
    "  \\rho & \\rho=1 & \\rho'&\n",
    " \\end{Bmatrix}\n",
    "\\chi\\begin{Bmatrix}\n",
    "  S_- & \\frac{1}{2} & S'_- \\\\\n",
    "  S_+ & \\frac{1}{2} & S'_+ \\\\\n",
    "  S & S_o & S' \\\\\n",
    " \\end{Bmatrix}(-1)^{\\eta+\\frac{1}{2}+S_+-S'_++\\lambda'_+-\\lambda_++\\mu'_+-\\mu_+}\\sqrt{\\frac{\\text{dim}(\\lambda_+\\mu_+)}{\\text{dim}(\\lambda'_+\\mu'_+)}}\\frac{\\sqrt{2S_++1}}{\\sqrt{2S'_++1}}\n",
    "\\\\\\\\ \\times\\Big\\langle[f'_-],(\\lambda'_-\\mu'_-),S'_-\\Big|\\Big|\\Big|a^{\\dagger}_{(\\eta'0)\\frac{1}{2}}\\Big|\\Big|\\Big| [f_-],(\\lambda_-\\mu_-)S_-\\Big\\rangle_{\\rho=1}\n",
    "\\Big\\langle[f_+],(\\lambda_+\\mu_+),S_+\\Big|\\Big|\\Big|a^{\\dagger}_{(\\eta0)\\frac{1}{2}}\\Big|\\Big|\\Big|[f'_+],(\\lambda'_+\\mu'_+),S'_+\\Big\\rangle_{\\rho=1}\n",
    "}\n",
    "$$  \n",
    "  "
   ]
  },
  {
   "cell_type": "markdown",
   "id": "c1dd3e70",
   "metadata": {},
   "source": [
    "# 2. Upwards transition $\\eta<\\eta'$\n"
   ]
  },
  {
   "cell_type": "markdown",
   "id": "3ce9d2c1",
   "metadata": {},
   "source": [
    "Similar proceedure but the following symmetry relations must be applied in order to construct the $9-j$ and $9-(\\lambda\\mu)$ coefficients\n",
    "\n",
    "$$\n",
    "\\langle \\frac{1}{2},m_{s'},\\frac{1}{2},m_{s}|S_o,M_{S_o}\\rangle = (-1)^{1-S_o}\\langle \\frac{1}{2},m_{s},\\frac{1}{2},m_{s'}|S_o,M_{S_o}\\rangle\n",
    "$$\n",
    "\n",
    "$$\n",
    "\\langle l',m_{l'},l,m_{l}|L_o,M_{L_o}\\rangle = (-1)^{l+l'-L_o}\\langle l,m_{l},l',m_{l'}|L_o,M_{L_o}\\rangle\n",
    "$$\n",
    "\n",
    "$$\n",
    "\\langle(\\eta',0),0,l'; (0,\\eta),0,l||(\\lambda_o\\mu_o),K_o,L_o\\rangle_{\\rho_o=1} = (-1)^{\\eta'+\\eta-\\lambda_o-\\mu_o+l+l'-L_o}\\langle(0,\\eta),0,l; (\\eta',0),0,l'||(\\lambda_o\\mu_o),K_o,L_o\\rangle_{\\rho_o=1}\n",
    "$$\n",
    "\n",
    "resulting in\n",
    "\n",
    "abvoe which results in \n",
    "    \n",
    "$$  \n",
    "\\boxed{\n",
    "\\Big\\langle[f'_-]\\otimes[f'_+],(\\lambda'_-\\mu'_-)\\otimes(\\lambda'_+\\mu'_+),\\rho'(\\lambda'\\mu'),S'\\Big|\\Big|\\Big| \\big\\{a^{\\dagger}_{(\\eta'0)\\frac{1}{2}}\\tilde{a}_{(0\\eta)\\frac{1}{2}}\\big\\}^{\\rho_0=1,(\\lambda_0\\mu_0)S_0}\\Big|\\Big|\\Big|[f_-]\\otimes[f_+],(\\lambda_-\\mu_-)\\otimes(\\lambda_+\\mu_+),\\rho(\\lambda\\mu),S\\Big\\rangle_{\\bar{\\rho}}\n",
    "\\\\= \\begin{Bmatrix}\n",
    "  (\\lambda_-,\\mu_-) & (0,\\eta) & (\\lambda'_-,\\mu'_-) & \\rho=1\\\\\n",
    "  (\\lambda_+,\\mu_+) & (\\eta',0) & (\\lambda'_+,\\mu'_+) & \\rho=1\\\\\n",
    "  (\\lambda,\\mu) & (\\lambda_o,\\mu_o) & (\\lambda',\\mu') & \\bar{\\rho}\\\\\n",
    "  \\rho & \\rho=1 & \\rho'&\n",
    " \\end{Bmatrix}\n",
    "\\chi\\begin{Bmatrix}\n",
    "  S_- & \\frac{1}{2} & S'_- \\\\\n",
    "  S_+ & \\frac{1}{2} & S'_+ \\\\\n",
    "  S & S_o & S' \\\\\n",
    " \\end{Bmatrix}(-1)^{\\eta'+\\frac{3}{2}+S_--S'_--S_o+\\lambda'_-+\\mu'_--\\lambda_--\\mu_--\\lambda_o-\\mu_o}\\sqrt{\\frac{\\text{dim}(\\lambda_-\\mu_-)}{\\text{dim}(\\lambda'_-\\mu'_-)}}\\frac{\\sqrt{2S_-+1}}{\\sqrt{2S'_-+1}}\n",
    "\\\\\\\\ \\times\\Big\\langle[f'_+],(\\lambda'_+\\mu'_+),S'_+\\Big|\\Big|\\Big|a^{\\dagger}_{(\\eta'0)\\frac{1}{2}}\\Big|\\Big|\\Big| [f_+],(\\lambda_+\\mu_+)S_+\\Big\\rangle_{\\rho=1}\n",
    "\\Big\\langle[f_-],(\\lambda_-\\mu_-),S_-\\Big|\\Big|\\Big|a^{\\dagger}_{(\\eta0)\\frac{1}{2}}\\Big|\\Big|\\Big|[f'_-],(\\lambda'_-\\mu'_-),S'_-\\Big\\rangle_{\\rho=1}\n",
    "}\n",
    "$$  \n",
    "  "
   ]
  },
  {
   "cell_type": "markdown",
   "id": "67f273c1",
   "metadata": {},
   "source": [
    "# 3. Relation between $\\Big\\langle[f''](\\lambda''\\mu''),S''\\Big|\\Big|\\Big|\\tilde{a}_{(0\\eta)\\frac{1}{2}}\\Big|\\Big|\\Big|[f](\\lambda\\mu),S\\Big\\rangle_{\\rho_2=1}$ and $\\Big\\langle[f](\\lambda\\mu),S\\Big|\\Big|\\Big|a^{\\dagger}_{(\\eta0)\\frac{1}{2}}\\Big|\\Big|\\Big|[f''](\\lambda''\\mu''),S''\\Big\\rangle_{\\rho_1=1}$\n",
    "    \n",
    "$$\\Big\\langle[f''](\\lambda''\\mu''),K'',L'',M_{L''},S'',M_{S''}\\Big|\\tilde{a}_{(0\\eta)lm_l\\frac{1}{2}m_s}\\Big|[f](\\lambda\\mu),K,L,M_{L},S,M_{S}\\Big\\rangle\\\\\n",
    "=\\langle LM_{L}lm_{l}|L''M_{L''}\\rangle\n",
    "\\langle SM_{S}\\frac{1}{2}m_{s}|S''M_{S''}\\rangle\n",
    "\\langle(\\lambda\\mu),K,L;(0\\eta)0l ||(\\lambda''\\mu''),K'',L''\\rangle_{\\rho=1} \\Big\\langle[f''](\\lambda''\\mu''),S''\\Big|\\Big|\\Big|\\tilde{a}_{(0\\eta)\\frac{1}{2}}\\Big|\\Big|\\Big|[f](\\lambda\\mu),S\\Big\\rangle_{\\rho=1}\\\\\n",
    "=\\Big\\langle[f](\\lambda\\mu),K,L,M_{L},S,M_{S}\\Big|(-1)^{\\eta+l-m_l+\\frac{1}{2}-m_s}a^{\\dagger}_{(\\eta0)l-m_{l}\\frac{1}{2}-m_{s}}\\Big|[f''](\\lambda''\\mu''),K'',L'',M_{L''},S'',M_{S''}\\Big\\rangle\\\\\n",
    "= (-1)^{\\eta+l-m_l+\\frac{1}{2}-m_s}\\langle L''M_{L''}l-m_{l}|LM_{L}\\rangle\n",
    "\\langle S''M_{S''}\\frac{1}{2}-m_{s}|SM_{S}\\rangle\\langle(\\lambda''\\mu'')K''L'';(\\eta0)0l ||(\\lambda\\mu)KL\\rangle_{\\rho=1}\\\\ \\times\\Big\\langle[f](\\lambda\\mu),S\\Big|\\Big|\\Big|a^{\\dagger}_{(\\eta0)\\frac{1}{2}}\\Big|\\Big|\\Big|[f''](\\lambda''\\mu''),S''\\Big\\rangle_{\\rho=1}\n",
    "$$\n",
    " \n",
    "\n"
   ]
  },
  {
   "cell_type": "markdown",
   "id": "9da54a24",
   "metadata": {},
   "source": [
    "<li> Apply $\\langle L''M_{L''}l-m_{l}|LM_{L}\\rangle = (-1)^{L+M_{L}-L''-M_{L^{''}}}\\sqrt{\\frac{2L+1}{2L''+1}}\\langle LM_{L}lm_{l}|L''M_{L''}\\rangle$ and $\\langle S''M_{S''}\\frac{1}{2}-m_{s}|SM_{S}\\rangle = (-1)^{S+M_{S}-S''-M_{S^{''}}}\\sqrt{\\frac{2S+1}{2S''+1}}\\langle SM_{S}\\frac{1}{2}m_{s}|S''M_{S''}\\rangle$. Simplify the Clebsch-Gordan coefficients\n",
    "    \n",
    "$$\\langle(\\lambda\\mu),K,L;(0\\eta)0l ||(\\lambda''\\mu''),K'',L''\\rangle_{\\rho=1} \\Big\\langle[f''](\\lambda''\\mu''),S''\\Big|\\Big|\\Big|\\tilde{a}_{(0\\eta)\\frac{1}{2}}\\Big|\\Big|\\Big|[f](\\lambda\\mu),S\\Big\\rangle_{\\rho=1}\\\\\n",
    "= (-1)^{\\eta+l-m_l+\\frac{1}{2}-m_s+L+M_{L}-L''-M_{L^{''}}+S+M_{S}-S''-M_{S^{''}}}\\langle(\\lambda''\\mu'')K''L'';(\\eta0)0l ||(\\lambda\\mu)KL\\rangle_{\\rho=1} \\sqrt{\\frac{2L+1}{2L''+1}} \\sqrt{\\frac{2S+1}{2S''+1}}\\\\\\times \\Big\\langle[f](\\lambda\\mu),S\\Big|\\Big|\\Big|a^{\\dagger}_{(\\eta0)\\frac{1}{2}}\\Big|\\Big|\\Big|[f''](\\lambda''\\mu''),S''\\Big\\rangle_{\\rho=1}\n",
    "$$"
   ]
  },
  {
   "cell_type": "markdown",
   "id": "0be2ff8b",
   "metadata": {},
   "source": [
    "\n",
    "<li> Apply symmetry relation $\\langle(\\lambda''\\mu'')K''L'';(\\eta0)0l ||(\\lambda\\mu)KL\\rangle_{\\rho=1} = (-1)^{\\lambda''-\\lambda+\\mu''-\\mu+L''+l-L}\\sqrt{\\frac{\\text{dim}(\\lambda\\mu)(2L''+1)}{\\text{dim}(\\lambda''\\mu'')(2L+1)}}\\langle(\\lambda\\mu)KL;(0\\eta)0l ||(\\lambda''\\mu'')K''L''\\rangle_{\\rho=1}$. Cancel the $SU(3)$ coefficients and simplify the phase.\n",
    "    \n",
    "$$\\Big\\langle[f''](\\lambda''\\mu''),S''\\Big|\\Big|\\Big|\\tilde{a}_{(0\\eta)\\frac{1}{2}}\\Big|\\Big|\\Big|[f](\\lambda\\mu),S\\Big\\rangle_{\\rho=1}\\\\\n",
    "= (-1)^{\\eta+l-m_l+\\frac{1}{2}-m_s+L+M_{L}-L''-M_{L^{''}}+S+M_{S}-S''-M_{S^{''}}}(-1)^{\\lambda''-\\lambda+\\mu''-\\mu+L''+l-L}\\sqrt{\\frac{\\text{dim}(\\lambda\\mu)}{\\text{dim}(\\lambda''\\mu'')}}\\sqrt{\\frac{2S+1}{2S''+1}}\\Big\\langle[f](\\lambda\\mu),S\\Big|\\Big|\\Big|a^{\\dagger}_{(\\eta0)\\frac{1}{2}}\\Big|\\Big|\\Big|[f''](\\lambda''\\mu''),S''\\Big\\rangle_{\\rho=1}\\\\\n",
    "= (-1)^{\\eta+\\frac{1}{2}+S-S''+\\lambda''-\\lambda+\\mu''-\\mu}\\sqrt{\\frac{\\text{dim}(\\lambda\\mu)}{\\text{dim}(\\lambda''\\mu'')}}\\sqrt{\\frac{2S+1}{2S''+1}}\\Big\\langle[f](\\lambda\\mu),S\\Big|\\Big|\\Big|a^{\\dagger}_{(\\eta0)\\frac{1}{2}}\\Big|\\Big|\\Big|[f''](\\lambda''\\mu''),S''\\Big\\rangle_{\\rho=1}\n",
    "$$\n",
    "    \n",
    "<li> Result:\n",
    "    \n",
    "$$\\boxed{\\Big\\langle[f''](\\lambda''\\mu''),S''\\Big|\\Big|\\Big|\\tilde{a}_{(0\\eta)\\frac{1}{2}}\\Big|\\Big|\\Big|[f](\\lambda\\mu),S\\Big\\rangle_{\\rho=1}\n",
    "= (-1)^{\\eta+\\frac{1}{2}+S-S''+\\lambda''-\\lambda+\\mu''-\\mu}\\sqrt{\\frac{\\text{dim}(\\lambda\\mu)}{\\text{dim}(\\lambda''\\mu'')}}\\sqrt{\\frac{2S+1}{2S''+1}}\\Big\\langle[f](\\lambda\\mu),S\\Big|\\Big|\\Big|a^{\\dagger}_{(\\eta0)\\frac{1}{2}}\\Big|\\Big|\\Big|[f''](\\lambda''\\mu''),S''\\Big\\rangle_{\\rho=1}}\n",
    "$$\n",
    "\n"
   ]
  }
 ],
 "metadata": {
  "kernelspec": {
   "display_name": "Python 3 (ipykernel)",
   "language": "python",
   "name": "python3"
  },
  "language_info": {
   "codemirror_mode": {
    "name": "ipython",
    "version": 3
   },
   "file_extension": ".py",
   "mimetype": "text/x-python",
   "name": "python",
   "nbconvert_exporter": "python",
   "pygments_lexer": "ipython3",
   "version": "3.9.12"
  }
 },
 "nbformat": 4,
 "nbformat_minor": 5
}
